

## fast\_fibonacci

October 4, 2021

```
[1]: from sympy import *
```

Consider Fibonacci numbers  $F_n$ :  $F_0 = 0, F_1 = 1, F_{n+2} = F_n + F_{n+1}$ .

```
[2]: def F(n):  
    if n == 0:  
        return 0  
    if n <= 2:  
        return 1  
    return F(n-1) + F(n-2)  
  
[F(n) for n in range(11)]
```

```
[2]: [0, 1, 1, 2, 3, 5, 8, 13, 21, 34, 55]
```

Denote  $\Phi_{n+1} := \begin{bmatrix} F_{n+1} \\ F_n \end{bmatrix}$

Then  $\Phi_{n+2} = \begin{bmatrix} F_{n+2} \\ F_{n+1} \end{bmatrix} = \begin{bmatrix} F_{n+1} + F_n \\ F_{n+1} \end{bmatrix} = \begin{bmatrix} 1 & 1 \\ 1 & 0 \end{bmatrix} \cdot \begin{bmatrix} F_{n+1} \\ F_n \end{bmatrix} = \begin{bmatrix} 1 & 1 \\ 1 & 0 \end{bmatrix} \cdot \Phi_{n+1}$

So  $\Phi_{n+1} = \begin{bmatrix} 1 & 1 \\ 1 & 0 \end{bmatrix} \cdot \Phi_n$

Denote  $A := \begin{bmatrix} 1 & 1 \\ 1 & 0 \end{bmatrix}$

Then  $\Phi_{n+1} = A \cdot \Phi_n = A^n \cdot \Phi_1 = A^n \cdot \begin{bmatrix} 1 \\ 0 \end{bmatrix}$

Notice, that  $A^n$  has form  $\begin{bmatrix} p+q & q \\ q & p \end{bmatrix}$  for all natural  $n$

Let's check it by induction

```
[3]: p = IndexedBase('p')  
q = IndexedBase('q')  
m, n = symbols('m, n')
```

```
[4]: def A(n):  
    return Matrix([[p[n] + q[n], q[n]], [q[n], p[n]]])
```

[5]: `A(n)`

[5]: 
$$\begin{bmatrix} p_n + q_n & q_n \\ q_n & p_n \end{bmatrix}$$

Base case:

[6]: `A1 = A(1).subs({p[1]: 0, q[1]: 1}); A1`

[6]: 
$$\begin{bmatrix} 1 & 1 \\ 1 & 0 \end{bmatrix}$$

Induction step:

If  $A^n = \begin{bmatrix} p_i + q_i & q_i \\ q_i & p_i \end{bmatrix}$  for all natural  $i \leq n$

then  $A^n \cdot A = A^{n+1}$  with substitution  $p_{n+1} = q_n, q_{n+1} = p_n + q_n$

[7]: `A(n) * A1`

[7]: 
$$\begin{bmatrix} p_n + 2q_n & p_n + q_n \\ p_n + q_n & q_n \end{bmatrix}$$

[8]: `A(n+1).subs({p[n+1]: q[n], q[n+1]: p[n] + q[n]})`

[8]: 
$$\begin{bmatrix} p_n + 2q_n & p_n + q_n \\ p_n + q_n & q_n \end{bmatrix}$$

Now we can get  $\Phi_{n+1} = \begin{bmatrix} F_{n+1} \\ F_n \end{bmatrix} = A^n \cdot \Phi_1 = A^n \cdot \begin{bmatrix} 1 \\ 0 \end{bmatrix} = \begin{bmatrix} p_n + q_n & q_n \\ q_n & p_n \end{bmatrix} \cdot \begin{bmatrix} 1 \\ 0 \end{bmatrix}$

So  $F_n = q_n = p_{n+1}, F_{n+1} = p_n + q_n = q_{n+1}$

Let's compute  $A^{m+n}$  by coefficients of  $A^m$  and  $A^n$

[9]: `Amn = A(n) * A(m); Amn`

[9]: 
$$\begin{bmatrix} (p_m + q_m)(p_n + q_n) + q_m q_n & (p_n + q_n) q_m + p_m q_n \\ (p_m + q_m) q_n + p_n q_m & p_m p_n + q_m q_n \end{bmatrix}$$

[10]: `p_mn = Amn[1, 1]; p_mn`

[10]: 
$$p_m p_n + q_m q_n$$

[11]: `q_mn = Amn[0, 1]; q_mn`

[11]: 
$$(p_n + q_n) q_m + p_m q_n$$

Now we can use these formulas to fast compute of Fibonacci numbers (see `pmtests.lesson1.Fibonacci.fast()` method):

$$\begin{cases} p_{m+n} = p_m p_n + q_m q_n \\ q_{m+n} = (p_n + q_n) q_m + p_m q_n \end{cases}$$

Let's check its

```
[12]: pn = [0] # pn[i] = p_mn[i+1]
      qn = [1] # qn[i] = q_mn[i+1]

      for i in range(1, 10):
          pn.append(p_mn.subs({m: i, n: 1}))
          qn.append(q_mn.subs({m: i, n: 1}))
          for j in range(i):
              pn[i] = pn[i].subs({p[j+1]: pn[j], q[j+1]: qn[j]})
              qn[i] = qn[i].subs({p[j+1]: pn[j], q[j+1]: qn[j]})

      pn, qn
```

```
[12]: ([0, 1, 1, 2, 3, 5, 8, 13, 21, 34], [1, 1, 2, 3, 5, 8, 13, 21, 34, 55])
```

```
[13]: display(A1**2)
      Amn.subs({m: 1, n: 1, p[1]: pn[0], q[1]: qn[0]})
```

```
[13]: 
$$\begin{bmatrix} 2 & 1 \\ 1 & 1 \end{bmatrix}$$

```

```
[14]: display(A1**3)
      Amn.subs({m: 2, n: 1,
                  p[1]: pn[0], q[1]: qn[0],
                  p[2]: pn[1], q[2]: qn[1]})
```

```
[14]: 
$$\begin{bmatrix} 3 & 2 \\ 2 & 1 \end{bmatrix}$$

```

```
[15]: display(A1**4)
      Amn.subs({m: 2, n: 2,
                  p[1]: pn[0], q[1]: qn[0],
                  p[2]: pn[1], q[2]: qn[1]})
```

```
[15]: 
$$\begin{bmatrix} 5 & 3 \\ 3 & 2 \end{bmatrix}$$

```